Replace Solver by NewSolver

src/MicroSail/Symbolic/Mutator.v
@@ -500,234 +500,7 @@ Module Mutators
 
   End MultiSubs.
 
-  Section Solver.
-
-    Definition try_solve_eq {Σ σ} (t1 t2 : Term Σ σ) : option bool :=
-      if Term_eqb t1 t2
-      then Some true
-      else
-        (* If the terms are literals, we can trust the negative result. *)
-        match t1 , t2 with
-        | term_lit _ _ , term_lit _ _ => Some false
-        | term_inr _   , term_inl _   => Some false
-        | term_inl _   , term_inr _   => Some false
-        | _            , _            => None
-        end.
-
-    Lemma try_solve_eq_spec {Σ σ} (t1 t2 : Term Σ σ) :
-      OptionSpec
-        (fun b => forall ι, inst t1 ι = inst t2 ι <-> is_true b)
-        True
-        (try_solve_eq t1 t2).
-    Proof.
-      unfold try_solve_eq.
-      destruct (Term_eqb_spec t1 t2).
-      - constructor. intros. apply reflect_iff.
-        constructor. congruence.
-      - destruct t1; dependent elimination t2; constructor; auto;
-        intros; apply reflect_iff; constructor; cbn; congruence.
-    Qed.
-
-    (* Check if the given formula is always true or always false for any
-       assignments of the logic variables. *)
-    Definition try_solve_formula {Σ} (fml : Formula Σ) : option bool :=
-      match fml with
-      | formula_bool t =>
-        match t in Term _ σ return option (Lit σ)
-        with
-        | term_lit _ b => Some b
-        | _            => None
-        end
-      | formula_prop _ _ => None
-      | formula_eq t1 t2 => try_solve_eq t1 t2
-        (* else Term_eqvb t1 t2 *)
-      | formula_neq t1 t2 => option_map negb (try_solve_eq t1 t2)
-        (* else option_map negb (Term_eqvb t1 t2) *)
-      end.
-
-    Lemma try_solve_formula_spec {Σ} (fml : Formula Σ) :
-      OptionSpec
-        (fun b => forall ι, inst fml ι <-> is_true b)
-        True
-        (try_solve_formula fml).
-    Proof.
-      destruct fml; cbn.
-      - dependent elimination t; constructor; auto.
-      - constructor; auto.
-      - destruct (try_solve_eq_spec t1 t2); now constructor.
-      - destruct (try_solve_eq_spec t1 t2); constructor; auto.
-        intros ι. specialize (H ι). destruct a; intuition.
-    Qed.
-
-    (* Poor man's unification *)
-    Definition try_unify {w : World} {σ} (t1 t2 : Term w σ) :
-      option { w' & MultiSub w w' } :=
-      match t1 with
-      | @term_var _ ς σ ςInΣ =>
-        fun t2 : Term w σ =>
-          match occurs_check ςInΣ t2 with
-          | Some t => Some (existT _ (multisub_cons ς t multisub_id))
-          | None => None
-          end
-      | _ => fun _ => None
-      end t2.
-
-    Definition try_propagate {w : World} (fml : Formula w) :
-      option { w' & MultiSub w w' } :=
-      match fml with
-      | formula_eq t1 t2 =>
-        match try_unify t1 t2 with
-        | Some r => Some r
-        | None => try_unify t2 t1
-        end
-      | _ => None
-      end.
-
-    Lemma try_unify_spec {w : World} {σ} (t1 t2 : Term w σ) :
-      OptionSpec (fun '(existT w' ν) => forall ι, inst t1 ι = inst t2 ι <-> inst_multisub ν ι) True (try_unify t1 t2).
-    Proof.
-      unfold try_unify. destruct t1; cbn; try (constructor; auto; fail).
-      destruct (occurs_check ςInΣ t2) eqn:Heq; constructor; auto.
-      apply (occurs_check_sound (T := fun Σ => Term Σ _)) in Heq. subst.
-      intros ι. rewrite inst_subst, inst_sub_shift.
-      cbn. intuition.
-    Qed.
-
-    Lemma try_propagate_spec {w : World} (fml : Formula w) :
-      OptionSpec (fun '(existT w' ν) => forall ι, (inst fml ι : Prop) <-> inst_multisub ν ι) True (try_propagate fml).
-    Proof.
-      unfold try_propagate; destruct fml; cbn; try (constructor; auto; fail).
-      destruct (try_unify_spec t1 t2) as [[w' ν] HYP|_]. constructor. auto.
-      destruct (try_unify_spec t2 t1) as [[w' ν] HYP|_]. constructor.
-      intros ι. specialize (HYP ι). intuition.
-      now constructor.
-    Qed.
-
-    Open Scope lazy_bool_scope.
-    Equations(noind) formula_eqb {Σ} (f1 f2 : Formula Σ) : bool :=
-      formula_eqb (formula_bool t1) (formula_bool t2) := Term_eqb t1 t2;
-      formula_eqb (@formula_eq _ σ t11 t12) (@formula_eq _ τ t21 t22) with eq_dec σ τ => {
-        formula_eqb (@formula_eq _ σ t11 t12) (@formula_eq _ ?(σ) t21 t22) (left eq_refl) :=
-          Term_eqb t11 t21 &&& Term_eqb t12 t22;
-       formula_eqb (@formula_eq _ σ t11 t12) (@formula_eq _ τ t21 t22) (right _) := false
-      };
-      formula_eqb (@formula_neq _ σ t11 t12) (@formula_neq _ τ t21 t22) with eq_dec σ τ => {
-        formula_eqb (@formula_neq _ σ t11 t12) (@formula_neq _ ?(σ) t21 t22) (left eq_refl) :=
-          Term_eqb t11 t21 &&& Term_eqb t12 t22;
-        formula_eqb (@formula_neq _ σ t11 t12) (@formula_neq _ τ t21 t22) (right _) := false
-      };
-      formula_eqb _ _ := false.
-
-    Lemma formula_eqb_spec {Σ} (f1 f2 : Formula Σ) :
-      BoolSpec (f1 = f2) True (formula_eqb f1 f2).
-    Proof.
-      induction f1; dependent elimination f2;
-        simp formula_eqb;
-        try (constructor; auto; fail).
-      - destruct (Term_eqb_spec t t0); constructor; intuition.
-      - destruct (eq_dec σ σ0); cbn.
-        + destruct e.
-          repeat
-            match goal with
-            | |- context[Term_eqb ?t1 ?t2] =>
-              destruct (Term_eqb_spec t1 t2); cbn;
-                try (constructor; intuition; fail)
-            end.
-        + constructor; auto.
-      - destruct (eq_dec σ σ1); cbn.
-        + destruct e.
-          repeat
-            match goal with
-            | |- context[Term_eqb ?t1 ?t2] =>
-              destruct (Term_eqb_spec t1 t2); cbn;
-                try (constructor; intuition; fail)
-            end.
-        + constructor; auto.
-    Qed.
-
-    Fixpoint try_assumption {Σ} (pc : PathCondition Σ) (fml : Formula Σ) {struct pc} : bool :=
-      match pc with
-      | nil       => false
-      | cons f pc => formula_eqb f fml ||| try_assumption pc fml
-      end.
-
-    Lemma try_assumption_spec {Σ} (pc : PathCondition Σ) (fml : Formula Σ) :
-      BoolSpec (forall ι, instpc pc ι -> inst (A := Prop) fml ι) True (try_assumption pc fml).
-    Proof.
-      induction pc; cbn.
-      - constructor; auto.
-      - destruct (formula_eqb_spec a fml).
-        + subst a. constructor. intros ι.
-          rewrite inst_pathcondition_cons.
-          intuition.
-        + destruct IHpc.
-          * constructor. intros ι.
-            rewrite inst_pathcondition_cons.
-            intuition.
-          * constructor; auto.
-    Qed.
-
-    Definition solver {w0 : World} (fml : Formula w0) :
-      option { w1 & MultiSub w0 w1 * List Formula w1 }%type :=
-      match try_propagate fml with
-      | Some (existT Σ1 vareqs) => Some (existT Σ1 (vareqs , nil))
-      | None =>
-        match try_solve_formula fml with
-        | Some true => Some (existT w0 (multisub_id , nil))
-        | Some false => None
-        | None =>
-          if try_assumption (wco w0) fml
-          then Some (existT w0 (multisub_id , nil))
-          else Some (existT w0 (multisub_id , (cons fml nil)))
-        end
-      end.
-
-    Lemma solver_spec {w0 : World} (fml : Formula w0) :
-      OptionSpec
-        (fun '(existT Σ1 (ζ, fmls)) =>
-           forall ι0,
-             instpc (wco w0) ι0 ->
-             (inst (A:= Prop) fml ι0 -> inst_multisub ζ ι0) /\
-             (forall ι1,
-                 ι0 = inst (wsub (wmultisub_sup ζ)) ι1 ->
-                 inst fml ι0 <-> inst fmls ι1))
-        (forall ι, instpc (wco w0) ι -> inst (A := Prop) fml ι -> False)
-        (solver fml).
-    Proof.
-      unfold solver.
-      destruct (try_propagate_spec fml) as [[Σ1 ζ01]|].
-      { constructor. intros ι0 Hpc. specialize (H ι0).
-        split. intuition. intros ι1 ->.
-        intuition. constructor. clear H. apply H1.
-        apply inst_multisub_inst_sub_multi.
-      }
-      clear H.
-      destruct (try_solve_formula_spec fml) as [b|].
-      { destruct b.
-        - constructor. intros ι0 Hpc. cbn. split; auto.
-          intros ? Hι. rewrite inst_sub_id in Hι. subst ι1.
-          specialize (H ι0). intuition. constructor.
-        - constructor. unfold is_true in H. intuition.
-      }
-      clear H.
-      destruct (try_assumption_spec (wco w0) fml).
-      { constructor. intros ι0 Hpc. specialize (H ι0).
-        cbn. split; auto. intros ι1 ->.
-        rewrite inst_sub_id in *. intuition.
-        constructor.
-      }
-      clear H.
-      { constructor. intros ι0 Hpc. split.
-        cbn; auto. intros ι1 ->.
-        rewrite inst_pathcondition_cons.
-        cbn. rewrite inst_sub_id.
-        intuition. constructor.
-      }
-    Qed.
-
-  End Solver.
-
-  Module NewSolver.
+  Module Solver.
 
     Equations(noeqns) simplify_formula_bool {Σ} (t : Term Σ ty_bool) (k : List Formula Σ) : option (List Formula Σ) :=
     | term_var ς                | k := Some (cons (formula_bool (term_var ς)) k);
@@ -1193,7 +966,7 @@ Module Mutators
         now rewrite inst_multi.
     Qed.
 
-  End NewSolver.
+  End Solver.
 
   Module SPath.
 
@@ -2244,7 +2017,7 @@ Module Mutators
     Definition assume_formula :
       ⊢ Formula -> SDijkstra Unit :=
       fun w0 fml POST =>
-        match NewSolver.solver (cons fml nil) with
+        match Solver.solver (cons fml nil) with
         | Some (existT w1 (ν , fmls)) =>
           (* Assume variable equalities and the residual constraints *)
           assume_multisub ν
@@ -2264,7 +2037,7 @@ Module Mutators
     Definition assert_formula :
       ⊢ Message -> Formula -> SDijkstra Unit :=
       fun w0 msg fml POST =>
-        match NewSolver.solver (cons fml nil) with
+        match Solver.solver (cons fml nil) with
         | Some (existT w1 (ν , fmls)) =>
           (* Assert variable equalities and the residual constraints *)
           assert_multisub msg ν
